fstar/new/MLS.TreeSync.Extensions.fst
@@ -1,0 +1,157 @@
+module MLS.TreeSync.Extensions
+
+open Lib.IntTypes
+open Lib.ByteSequence
+open Lib.LoopCombinators
+open MLS.NetworkTypes
+open MLS.Parser
+open MLS.Result
+
+#set-options "--fuel 0 --ifuel 0"
+
+(*** Extensions parser ***)
+
+type capabilities_ext_nt = {
+  cen_versions: blseq protocol_version_nt ps_protocol_version ({min=0; max=255});
+  cen_ciphersuites: blseq cipher_suite_nt ps_cipher_suite ({min=0; max=255});
+  cen_extensions: blseq extension_type_nt ps_extension_type ({min=0; max=255});
+}
+
+#push-options "--ifuel 1"
+val ps_capabilities_ext: parser_serializer capabilities_ext_nt
+let ps_capabilities_ext =
+  let open MLS.Parser in
+  isomorphism capabilities_ext_nt
+    (
+      _ <-- ps_seq _ ps_protocol_version;
+      _ <-- ps_seq _ ps_cipher_suite;
+      ps_seq _ ps_extension_type
+    )
+    (fun (|versions, (|ciphersuites, extensions|)|) -> {
+      cen_versions = versions;
+      cen_ciphersuites = ciphersuites;
+      cen_extensions = extensions;
+    })
+    (fun x -> (|x.cen_versions, (|x.cen_ciphersuites, x.cen_extensions|)|))
+#pop-options
+
+type lifetime_ext_nt = {
+  len_not_before: uint64;
+  len_not_after: uint64;
+}
+
+val ps_lifetime_ext: parser_serializer lifetime_ext_nt
+let ps_lifetime_ext =
+  let open MLS.Parser in
+  isomorphism lifetime_ext_nt
+    (
+      _ <-- ps_u64;
+      ps_u64
+    )
+    (fun (|not_before, not_after|) -> {
+      len_not_before = not_before;
+      len_not_after = not_after;
+    })
+    (fun x -> (|x.len_not_before, x.len_not_after|))
+
+type key_package_identifier_ext_nt = {
+  kpien_key_id: blbytes ({min=0; max=(pow2 16)-1});
+}
+
+val ps_key_package_identifier_ext: parser_serializer key_package_identifier_ext_nt
+let ps_key_package_identifier_ext =
+  let open MLS.Parser in
+  isomorphism key_package_identifier_ext_nt (ps_bytes _)
+    (fun key_id -> {kpien_key_id = key_id})
+    (fun x -> x.kpien_key_id)
+
+type parent_hash_ext_nt = {
+  phen_parent_hash: blbytes ({min=0; max=255});
+}
+
+val ps_parent_hash_ext: parser_serializer parent_hash_ext_nt
+let ps_parent_hash_ext =
+  let open MLS.Parser in
+  isomorphism parent_hash_ext_nt (ps_bytes _)
+    (fun key_id -> {phen_parent_hash = key_id})
+    (fun x -> x.phen_parent_hash)
+
+(*** Utility functions ***)
+
+val find_extension_index: extension_type_nt -> extensions:Seq.seq extension_nt -> option (i:nat{i < Seq.length extensions})
+let find_extension_index t extensions =
+  repeati (Seq.length extensions) (fun i acc ->
+    if (Seq.index extensions i).en_extension_type = t then
+      Some i
+    else
+      acc
+  ) None
+
+val get_extension: extension_type_nt -> bytes -> option bytes
+let get_extension t extensions_buf =
+  match (ps_to_pse (ps_seq ({min=8; max=(pow2 32)-1}) ps_extension)).parse_exact extensions_buf with
+  | None -> None
+  | Some extensions ->
+    match find_extension_index t extensions with
+    | None -> None
+    | Some i -> Some ((Seq.index extensions i).en_extension_data)
+
+val set_extension: extension_type_nt -> bytes -> bytes -> result bytes
+let set_extension t extensions_buf data =
+  extensions <-- from_option "set_extension: invalid extensions buffer" ((ps_to_pse (ps_seq ({min=8; max=(pow2 32)-1}) ps_extension)).parse_exact extensions_buf);
+  if not (Seq.length data < pow2 16) then
+    error "set_extension: data is too long"
+  else (
+    let ext = ({en_extension_type = t; en_extension_data = data;}) in
+    let new_extensions: Seq.seq extension_nt =
+      match find_extension_index t extensions with
+      | None -> Seq.append extensions (Seq.create 1 ext)
+      | Some i -> (Seq.upd extensions i ext)
+    in
+    let ext_byte_length = byte_length ps_extension (Seq.seq_to_list new_extensions) in
+    if not (8 <= ext_byte_length) then
+      error "set_extension: new extension buffer is too short"
+    else if not (ext_byte_length < pow2 32) then
+      error "set_extension: new extension buffer is too long"
+    else (
+      return ((ps_seq ({min=8; max=(pow2 32)-1}) ps_extension).serialize new_extensions)
+    )
+  )
+
+val mk_get_extension: #a:Type0 -> extension_type_nt -> parser_serializer a -> bytes -> option a
+let mk_get_extension #a ext_type ps_a buf =
+  match get_extension ext_type buf with
+  | None -> None
+  | Some res ->
+    (ps_to_pse ps_a).parse_exact res
+
+val mk_set_extension: #a:Type0 -> extension_type_nt -> parser_serializer a -> bytes -> a -> result bytes
+let mk_set_extension #a ext_type ps_a buf ext_content =
+  set_extension ext_type buf (ps_a.serialize ext_content)
+
+(*** Exposed functions ***)
+
+val get_extension_list: bytes -> result (list extension_type_nt)
+let get_extension_list extensions_buf =
+  extensions <-- from_option "set_extension: invalid extensions buffer" ((ps_to_pse (ps_seq ({min=8; max=(pow2 32)-1}) ps_extension)).parse_exact extensions_buf);
+  return (List.Tot.map (fun x -> x.en_extension_type) (Seq.seq_to_list extensions))
+
+val get_capabilities_extension: bytes -> option capabilities_ext_nt
+let get_capabilities_extension = mk_get_extension ET_capabilities ps_capabilities_ext
+val set_capabilities_extension: bytes -> capabilities_ext_nt -> result bytes
+let set_capabilities_extension = mk_set_extension ET_capabilities ps_capabilities_ext
+
+val get_lifetime_extension: bytes -> option lifetime_ext_nt
+let get_lifetime_extension = mk_get_extension ET_lifetime ps_lifetime_ext
+val set_lifetime_extension: bytes -> lifetime_ext_nt -> result bytes
+let set_lifetime_extension = mk_set_extension ET_lifetime ps_lifetime_ext
+
+val get_key_package_identifier_extension: bytes -> option key_package_identifier_ext_nt
+let get_key_package_identifier_extension = mk_get_extension ET_key_id ps_key_package_identifier_ext
+val set_key_package_identifier_extension: bytes -> key_package_identifier_ext_nt -> result bytes
+let set_key_package_identifier_extension = mk_set_extension ET_key_id ps_key_package_identifier_ext
+
+val get_parent_hash_extension: bytes -> option parent_hash_ext_nt
+let get_parent_hash_extension = mk_get_extension ET_parent_hash ps_parent_hash_ext
+val set_parent_hash_extension: bytes -> parent_hash_ext_nt -> result bytes
+let set_parent_hash_extension = mk_set_extension ET_parent_hash ps_parent_hash_ext
