fstar/new/MLS.TreeSync.IntegrityCheck.fst
@@ -1,0 +1,194 @@
+module MLS.TreeSync.IntegrityCheck
+
+open Lib.ByteSequence
+open MLS.Crypto
+open MLS.Parser
+open MLS.Result
+open MLS.Tree
+open MLS.TreeSync
+open MLS.TreeSync.Types
+open MLS.NetworkBinder
+open MLS.NetworkTypes
+open MLS.TreeSync.Extensions
+open MLS.TreeSync.ParentHash
+open MLS.TreeKEM.Types
+open MLS.TreeSyncTreeKEMBinder
+
+#set-options "--fuel 0 --ifuel 0"
+
+type leaf_integrity_error =
+  | LIE_BadSignature
+  | LIE_NoCapabilities
+  | LIE_ExtensionsNotInCapabilities
+  | LIE_NoLifetime
+
+type node_integrity_error =
+  | NIE_BadParentHash
+
+type integrity_error =
+  | IE_LeafError: leaf_integrity_error -> leaf_index:nat -> integrity_error
+  | IE_NodeError: node_integrity_error -> nb_left_leaves:nat -> level:nat -> integrity_error
+
+type integrity_either =
+  | IE_Good: integrity_either
+  | IE_Errors: list integrity_error -> integrity_either
+
+#push-options "--ifuel 1"
+private val op_Amp_Amp_Amp: integrity_either -> integrity_either -> integrity_either
+let op_Amp_Amp_Amp i1 i2 =
+  match i1, i2 with
+  | IE_Good, _ -> i2
+  | IE_Errors l1, IE_Good -> i1
+  | IE_Errors l1, IE_Errors l2 -> IE_Errors (l1@l2)
+#pop-options
+
+val integrity_either_to_bool: integrity_either -> bool
+let integrity_either_to_bool ie =
+  match ie with
+  | IE_Good -> true
+  | _ -> false
+
+val check_signature: ciphersuite -> leaf_package_t -> result (option leaf_integrity_error)
+let check_signature cs lp =
+  if not (Seq.length lp.lp_credential.cred_signature_key = sign_public_key_length cs) then
+    error "check_leaf_package: signature key has wrong length"
+  else if not (Seq.length lp.lp_signature = sign_signature_length cs) then
+    error "check_leaf_package: signature has wrong length"
+  else (
+    key_package <-- treesync_to_keypackage cs lp;
+    let leaf_package_bytes = ps_key_package_tbs.serialize (key_package_get_tbs key_package) in
+    if sign_verify cs lp.lp_credential.cred_signature_key leaf_package_bytes lp.lp_signature then
+      return None
+    else
+      return (Some LIE_BadSignature)
+  )
+
+val check_capabilities: leaf_package_t -> result (option leaf_integrity_error)
+let check_capabilities lp =
+  extensions_list <-- get_extension_list lp.lp_extensions;
+  let opt_capabilities_extension = get_capabilities_extension lp.lp_extensions in
+  return (
+    match opt_capabilities_extension with
+    | None -> Some LIE_NoCapabilities
+    | Some capabilities ->
+      let extension_inclusion = (
+        List.Tot.for_all (fun ext_type ->
+          List.Tot.mem ext_type (Seq.seq_to_list capabilities.cen_extensions)
+        ) extensions_list
+      ) in
+      if extension_inclusion then None
+      else Some LIE_ExtensionsNotInCapabilities
+  )
+
+val check_lifetime: leaf_package_t -> result (option leaf_integrity_error)
+let check_lifetime lp =
+  let opt_lifetime_extension = get_lifetime_extension lp.lp_extensions in
+  return (
+    match opt_lifetime_extension with
+    | None -> Some LIE_NoLifetime
+    | Some lifetime ->
+      None //TODO
+  )
+
+val convert_opt_leaf_error_to_either: option leaf_integrity_error -> nat -> integrity_either
+let convert_opt_leaf_error_to_either opt leaf_index =
+  match opt with
+  | None -> IE_Good
+  | Some x -> IE_Errors [IE_LeafError x leaf_index]
+
+val check_leaf: #l:nat -> #n:tree_size l -> ciphersuite -> nat -> t:treesync l n{TLeaf? t} -> result integrity_either
+let check_leaf #l #n cs leaf_index t =
+  let (TLeaf (_, olp)) = t in
+  match olp with
+  | None -> return IE_Good
+  | Some lp -> (
+    signature_check <-- check_signature cs lp;
+    capabilities_check <-- check_capabilities lp;
+    lifetime_check <-- check_lifetime lp;
+    let signature_either = convert_opt_leaf_error_to_either signature_check leaf_index in
+    let capabilities_either = convert_opt_leaf_error_to_either capabilities_check leaf_index in
+    let lifetime_either = convert_opt_leaf_error_to_either lifetime_check leaf_index in
+    return (signature_either &&& capabilities_either &&& lifetime_either)
+  )
+
+#push-options "--ifuel 1"
+val get_original_right_node: #l:nat -> #n:tree_size l -> treesync l n -> option (l_res:nat & n_res:tree_size l_res & treesync l_res n_res)
+let rec get_original_right_node #l #n t =
+  match t with
+  | TNode (_, Some np) _ _ ->
+    Some (|l, n, t|)
+  | TNode (_, None) left _ ->
+    get_original_right_node left
+  | TSkip _ t' ->
+    get_original_right_node t'
+  | TLeaf (_, Some lp) ->
+    Some (|l, n, t|)
+  | TLeaf (_, None) ->
+    None
+#pop-options
+
+#push-options "--ifuel 1"
+val get_parent_hash: #l:nat -> #n:tree_size l -> treesync l n -> option bytes
+let get_parent_hash #l #n t =
+  match t with
+  | TNode (_, None) _ _ -> None
+  | TNode (_, Some np) _ _ -> Some np.np_parent_hash
+  | TSkip _ _ -> None
+  | TLeaf (_, None) -> None
+  | TLeaf (_, Some lp) -> (
+    match get_parent_hash_extension lp.lp_extensions with
+    | Some parent_hash_ext -> Some (parent_hash_ext.phen_parent_hash)
+    | None -> None
+  )
+#pop-options
+
+#push-options "--ifuel 1"
+val check_internal_node: #l:nat -> #n:tree_size l -> ciphersuite -> nat -> t:treesync l n{TNode? t} -> result integrity_either
+let check_internal_node #l #n cs nb_left_leaves t =
+  let (TNode (_, onp) left right) = t in
+  match onp with
+  | None -> return IE_Good
+  | Some np -> (
+    public_key <-- (
+      kem_node_package <-- treesync_to_treekem_node_package cs nb_left_leaves np;
+      return kem_node_package.kp_public_key
+    );
+    parent_hash_from_left_ok <-- (
+      let real_parent_hash = get_parent_hash left in
+      computed_parent_hash <-- compute_parent_hash_from_dir cs public_key np.np_parent_hash nb_left_leaves t Left;
+      return (real_parent_hash = Some computed_parent_hash)
+    );
+    parent_hash_from_right_ok <-- (
+      match get_original_right_node right with
+      | None -> return false
+      | Some (|_, _, original_right|) -> (
+        let real_parent_hash = get_parent_hash original_right in
+        computed_parent_hash <-- compute_parent_hash_from_dir cs public_key np.np_parent_hash nb_left_leaves t Right;
+        return (real_parent_hash = Some computed_parent_hash)
+      )
+    );
+    if (parent_hash_from_left_ok || parent_hash_from_right_ok) then
+      return IE_Good
+    else
+      return (IE_Errors [IE_NodeError NIE_BadParentHash nb_left_leaves l])
+  )
+#pop-options
+
+#push-options "--ifuel 1"
+val check_treesync_aux: #l:nat -> #n:tree_size l -> ciphersuite -> nat -> treesync l n -> result integrity_either
+let rec check_treesync_aux #l #n cs nb_left_leaves t =
+  match t with
+  | TNode (_, onp) left right ->
+    left_ok <-- check_treesync_aux cs nb_left_leaves left;
+    right_ok <-- check_treesync_aux cs (nb_left_leaves + pow2 (l-1)) right;
+    cur_ok <-- check_internal_node cs nb_left_leaves t;
+    return (left_ok &&& cur_ok &&& right_ok)
+  | TSkip _ t' ->
+    check_treesync_aux cs nb_left_leaves t'
+  | TLeaf _ ->
+    check_leaf cs nb_left_leaves t
+#pop-options
+
+val check_treesync: #l:nat -> #n:tree_size l -> ciphersuite -> treesync l n -> result integrity_either
+let check_treesync #l #n cs t =
+  check_treesync_aux cs 0 t
